

⑤

A	$f_{A0}$	$-f_{A0} \frac{X}{2}$	$f_{A0}(1-X)$
B	0	$f_{A0} \frac{X}{2}$	$f_{A0} \frac{X}{2}$
C	$f_{C0}$	0	$f_{C0}$

$$f_T = f_{A0} + f_{C0} - f_{A0} \frac{X}{2}$$

$$f_T = f_{T0} - \frac{f_{A0}}{2f_{A0}} (f_{A0} - f_A)$$

$$f_T = f_{T0} - \frac{f_{A0}}{2} + \frac{f_A}{2}$$

$$\frac{f_T}{f_{T0}} = \left(1 - \frac{f_{A0}}{2f_{T0}}\right) + \frac{f_A}{2f_{T0}}$$

$$v = v_0 \left[ \left(1 - \frac{f_{A0}}{2f_{T0}}\right) + \frac{f_A}{2f_{T0}} \right]$$

$$\frac{df_A}{dv} = \frac{-K C_A^2 \cdot v^2}{v_0^2 \left[ \left(1 - \frac{f_{A0}}{2f_{T0}}\right) + \frac{f_A}{2f_{T0}} \right]^2}$$

$$\frac{df_A}{dv} = \frac{-K f_A^2}{v_0^2 \left[ \left(1 - \frac{f_{A0}}{2f_{T0}}\right) + \frac{f_A}{2f_{T0}} \right]^2}$$

$$\frac{v_0^2}{K} \int \left[ \frac{\left(1 - \frac{f_{A0}}{2f_{T0}}\right) + \frac{f_A}{2f_{T0}}}{f_A} \right]^2 df_A = -\int dv$$

equating this  
for I & II

\* assumed initial  $v_0$  as constant

Case I  $f_{T0} = 2f_{A0}$   $f_A \rightarrow f_{A0} \rightarrow 0.2f_{A0}$

Case II  $f_{T0} = \frac{3}{2}f_{A0}$   $f_A \rightarrow 0.5f_{A0}$ ?

$$\int_{0.2f_{A0}}^{f_{A0}} \left( \frac{\frac{3}{4} + \frac{f_A}{4f_{A0}}}{f_A} \right)^2 df_A = \int_{0.5f_{A0}}^{f_{A0}} \left( \frac{\frac{2}{3} + \frac{f_A}{3f_{A0}}}{f_A} \right)^2 df_A$$

$$\int_{0.2f_{A0}}^{f_{A0}} \left( \frac{3 + \frac{f_A}{f_{A0}}}{4f_A} \right)^2 df_A = \int_{f}^{0.5f_{A0}} \left( \frac{5 + \frac{f_A}{3f_{A0}}}{6f_A} \right)^2 df_A$$

$$f \approx 0.187 f_{A0}$$

$$X = \frac{0.5f_{A0} - 0.187f_{A0}}{0.5f_{A0}} = 0.626$$

62.6 % conversion.